Arithmetic Sequence Formula üëç

nth term is, an = a1 + (n - 1) d

Sum of n terms is, Sn = (n/2) [2a1 + (n - 1) d] 

(or)Sn =  (n/2) [a1 + an]

an = nth term,
a1 = first term, and
d is the common difference



:apple: Examples Using Arithmetic Sequence Formula ü•â üíØ
 
Example 1: Using the arithmetic sequence formula, find the 13th term in the sequence 1, 5, 9, 13...

Solution:

To find: 13th term of the given sequence.

Since the difference between consecutive terms is the same, the given sequence forms an arithmetic sequence.

a = 1, d = 4

Using arithmetic sequence formula,

an = a1+ (n - 1) d

For 13th term, n = 13

an = 1 + (13 - 1)4

an = 1 + (12)4

an = 1 + 48

an = 49

Answer: 13th term in the sequence is 49.


:anger: Example 2: Find the sum of the following arithmetic series: 3 + 7 + 11 + ....... (up to 25 terms).


To find the sum of the first 25 terms of the arithmetic sequence 3, 7, 11,.......

Given: a1 = 3, d = 4, n = 25

The given arithmetic sequence is 3, 7, 11,‚Ä¶.

Using the arithmetic series formula:

Sn = (n/2) [2a + (n - 1) d]

The sum of the first 25 terms

S25=(25/2) [2 x 3 + (25 - 1) 4]

= (25/2) [6 + 24 x 4]

= 25/2 √ó 102

= 1275

Answer: The sum of the given arithmetic series is 1275.